tla_crash_safe_disk_refinement.dfy
@@ -30,6 +30,7 @@ function DiskLog(k:Disk.Constants, s:Disk.Variables) : seq<Datum>
 // The view reflecting count operations.
 function IView(k:Constants, s:Variables, count:int) : AbstractMap.View
     requires Inv(k, s)
+    requires 0 <= count <= |s.memlog|
 {
     ILog(s.memlog[..count])
 }
@@ -40,13 +41,26 @@ function INumRunningViews(k:Constants, s:Variables) : int
     |s.memlog| - s.diskCommittedSize + 1
 }
 
-function {:opaque} IViewsDef(k:Constants, s:Variables, start:int, count:int) : (views:seq<AbstractMap.View>)
-    ensures forall i :: 0<=i<count ==> views[i] == IView(k, s, |s.memlog| - start + i)
+// Returns a sequence of views of s.memlog, from ..oldest+count-1 working backwards to ..oldest.
+// The IRunningViews common case is oldest==diskCommittedSize and count==INumRunningViews,
+// so the last entry is ..diskCommittedSize (the persistent view), and the first entry is
+// diskCommittedSize+|s.memlog|-diskCommittedSize+1-1 == |s.memlog| -- the whole log, or the
+// current ephemeral view.
+function {:opaque} IViewsDef(k:Constants, s:Variables, oldest:int, count:int) : (views:seq<AbstractMap.View>)
+    requires Inv(k, s)
+    requires 0 <= count
+    requires 0 <= oldest
+    requires oldest + count <= |s.memlog| + 1
+    ensures |views| == count
+    ensures forall i :: 0<=i<count ==> views[i] == IView(k, s, oldest + count - i - 1)
 {
-    if count==0 then [] else IViewsDef(k, s, start, count-1) + [IView(k, s, |s.memlog| - start + count - 1)]
+    assert oldest + count - 1 <= |s.memlog|;
+    if count==0 then [] else [IView(k, s, oldest + count - 1)] + IViewsDef(k, s, oldest, count-1)
 }
 
 function IRunningViews(k:Constants, s:Variables) : (views:seq<AbstractMap.View>)
+    requires Inv(k, s)
+    requires s.mode.Running?
 {
     IViewsDef(k, s, s.diskCommittedSize, INumRunningViews(k, s))
 }
@@ -59,6 +73,7 @@ function INotRunningView(k:Constants, s:Variables) : AbstractMap.View
 }
 
 function IViews(k:Constants, s:Variables) : seq<AbstractMap.View>
+    requires Inv(k, s)
 {
     if s.mode.Running?
     then IRunningViews(k, s)
@@ -66,25 +81,23 @@ function IViews(k:Constants, s:Variables) : seq<AbstractMap.View>
 }
 
 // Refinement to an AbstractMap
+function Ik(k:Constants) : AbstractMap.Constants
+{
+    AbstractMap.Constants()
+}
+
 function I(k:Constants, s:Variables) : AbstractMap.Variables
     requires Inv(k, s)
 {
     AbstractMap.Variables(IViews(k, s))
 }
 
-function Ik(k:Constants) : AbstractMap.Constants
-{
-    AbstractMap.Constants()
-}
-
-lemma InvImpliesRefinementInit(k:Constants, s:Variables)
-    requires Init(k, s)
-    ensures AbstractMap.Init(Ik(k), I(k, s))
+lemma EmptyILog()
+    ensures ILog([]) == AbstractMap.EmptyMap()
+    // Dafny bug: why can't I just stick this ensures on ILog defn?
 {
     reveal_ILog();
-    reveal_FindIndexInLog();
-//    assert IViews(k, s) == [AbstractMap.EmptyMap()];  // OBSERVE
-} 
+}
 
 lemma InvImpliesWF(k:Constants, s:Variables)
     requires Inv(k, s)
@@ -101,120 +114,32 @@ lemma LogAppend(log:seq<Datum>, datum:Datum)
     reveal_FindIndexInLog();
 }
 
-lemma PushLogNoop(k:Disk.Constants, s:Disk.Variables, s':Disk.Variables, len:int)
-    requires DiskLogPlausible(k, s)
-    requires DiskLogPlausible(k, s')
-    requires 0 <= len <= DiskLogSize(k, s)
-    requires forall i :: 0<=i<len ==> s.sectors[i] == s'.sectors[i] // OBSERVE, probably
-    ensures DiskLog(k, s') == DiskLog(k, s)
-
-function {:opaque} UpdateKeySet(log:seq<Datum>) : (keys:set<int>)
-    ensures forall i :: 0<=i<|log| ==> log[i].key in keys
-    ensures forall k, i :: 0<=i<|log| && !(k in keys) ==> log[i].key != k
-{
-    if log==[] then {} else UpdateKeySet(log[..|log|-1]) + {log[|log|-1].key}
-}
-
-function {:opaque} IndexForKey(log:seq<Datum>, key:int) : (idx:int)
-    requires key in UpdateKeySet(log)
-    ensures 0<=idx<|log|
-    ensures log[idx].key == key
-    ensures forall j :: idx < j < |log| ==> log[j].key != key
-{
-    reveal_UpdateKeySet();
-    if log[|log|-1].key == key
-    then |log|-1
-    else IndexForKey(log[..|log|-1], key)
-}
-
-lemma LogIndexFallThrough(log:seq<Datum>, logPrefix:seq<Datum>, logSuffix:seq<Datum>, k:int)
-    requires log == logPrefix + logSuffix
-    requires forall i :: 0<=i<|logSuffix| ==> logSuffix[i].key != k
-    ensures FindIndexInLog(log, k) == FindIndexInLog(logPrefix, k)
-    decreases |logSuffix|
-{
-    reveal_FindIndexInLog();
-    if logSuffix != [] {
-        var subSuffix := logSuffix[..|logSuffix|-1];
-        LogIndexFallThrough(logPrefix + subSuffix, logPrefix, subSuffix, k);
-        if |log| > 0 && log[|log|-1].key != k {
-            assert log[..|log|-1] == logPrefix + subSuffix;    // OBSERVE (sequences)
-        }
-    } else {
-        assert log == logPrefix;    // OBSERVE (sequences)
-    }
-}
-
-// If you don't find k in the suffix of a log, you can read the prefix.
-lemma LogFallThrough(log:seq<Datum>, logPrefix:seq<Datum>, logSuffix:seq<Datum>, k:int)
-    requires log == logPrefix + logSuffix
-    requires forall i :: 0<=i<|logSuffix| ==> logSuffix[i].key != k
-    ensures ILog(log)[k] == ILog(logPrefix)[k]
-{
-    reveal_ILog();
-    reveal_FindIndexInLog();
-    LogIndexFallThrough(log, logPrefix, logSuffix, k);
-}
-
-lemma PushLogMetadataRefinement(k:Constants, s:Variables, s':Variables)
-    requires LogImpl.PushLogMetadata(k, s, s')
+lemma AppendRefinement(k:Constants, s:Variables, s':Variables, datum:Datum)
     requires Inv(k, s)
-    ensures AbstractMap.WF(I(k, s))
-    ensures AbstractMap.WF(I(k, s'))
-    ensures AbstractMap.Next(Ik(k), I(k, s), I(k, s'))
+    requires NextStep(k, s, s', AppendStep(datum));
+    ensures AbstractMap.Next(Ik(k), I(k, s), I(k, s'));
 {
-    var Ik := Ik(k);
-    var Is := I(k, s);
-    var Is' := I(k, s');
-    var newIdxStart := s.diskCommittedSize;
-    var newIdxEnd := s.diskPersistedSize;   // exclusive
-    var logTail := s.disk.sectors[DiskLogAddr(newIdxStart) .. DiskLogAddr(newIdxEnd)];
-    var keys := UpdateKeySet(logTail);
-//    assert Is'.ephemeral == Is.ephemeral;
-    assert AbstractMap.WF(Is');
-//    forall key
-//        ensures Is'.persistent[key] == if key in keys then Is.ephemeral[key] else Is.persistent[key]
-//    {
-//        if key in keys {
-//            var suffixIdx := IndexForKey(logTail, key);
-//            var idx := newIdxStart + suffixIdx;
-//            var diskLog := DiskLog(k.disk, s'.disk);
-//
-//            assert FindIndexInLog(diskLog, key) == Some(idx);
-//
-//            assert |diskLog| == s'.diskCommittedSize;
-//            assert s'.diskCommittedSize == s.diskPersistedSize;
-//            assert s.diskPersistedSize == |s.memlog|;
-//            forall i | 0 <= i < s.diskPersistedSize
-//                ensures diskLog[i] == s.memlog[i]
-//            {
-//                assert Disk.Peek(k.disk, s.disk, DiskLogAddr(i), s.memlog[i]);
-//            }
-//
-//            assert diskLog == s.memlog;
-//            assert FindIndexInLog(s.memlog, key) == Some(idx);
-//            assert s.memlog[idx] == diskLog[idx];
-//            calc {
-//                IPersistent(k, s')[key];
-//                ILog(DiskLog(k.disk, s'.disk))[key];
-//                    { reveal_ILog(); }
-//                EvalLog(diskLog, key).value;
-//                EvalLog(s.memlog, key).value;
-//                    { reveal_ILog(); }
-//                IEphemeral(k, s)[key];
-//            }
-//            assert Is'.persistent[key] == Is.ephemeral[key];
-//        } else {
-//            var diskLog := DiskLog(k.disk, s.disk);
-//            var diskLog' := DiskLog(k.disk, s'.disk);
-//            var suffix := diskLog'[|diskLog|..];
-//            LogFallThrough(diskLog', diskLog, suffix, key);
-//            assert Is'.persistent[key] == Is.persistent[key];
-//        }
-//    }
-//    assert AbstractMap.PersistKeys(Ik, Is, Is', keys);
-//    assert AbstractMap.NextStep(Ik, Is, Is', AbstractMap.PersistKeysStep(keys));
+    var views' := IViewsDef(k, s', s'.diskCommittedSize, INumRunningViews(k, s'));
+    var views := IViewsDef(k, s, s.diskCommittedSize, INumRunningViews(k, s));
+    forall i | 0<=i<INumRunningViews(k, s)
+        ensures views'[i+1] == views[i]
+    {
+        var count := s.diskCommittedSize + INumRunningViews(k, s) - i - 1;
+        assert s'.memlog[..count] == s.memlog[..count]; // OBSERVE seqs
+    }
+    assert s'.memlog[..|s'.memlog|] == s'.memlog;   // OBSERVE seqs
+    assert s.memlog[..|s.memlog|] == s.memlog;  // OBSERVE seqs
+    LogAppend(s.memlog, datum);
+    assert AbstractMap.NextStep(Ik(k), I(k, s), I(k, s'), AbstractMap.WriteStep(datum)); // OBSERVE witness (Step)
 }
+
+lemma InvImpliesRefinementInit(k:Constants, s:Variables)
+    requires Init(k, s)
+    ensures AbstractMap.Init(Ik(k), I(k, s))
+{
+    EmptyILog();
+    assert IViews(k, s) == [AbstractMap.EmptyMap()];  // OBSERVE
+} 
 
 lemma InvImpliesRefinementNext(k:Constants, s:Variables, s':Variables)
     requires Next(k, s, s')
@@ -235,7 +160,10 @@ lemma InvImpliesRefinementNext(k:Constants, s:Variables, s':Variables)
 
     match step {
         case CrashAndRecover => {
-            assert AbstractMap.NextStep(Ik, Is, Is', AbstractMap.SpontaneousCrash);
+            if (s.mode.Running?) {
+                assert DiskLog(k.disk, s.disk) == s.memlog[..s.diskCommittedSize];  // OBSERVE
+            }
+            assert AbstractMap.NextStep(Ik, Is, Is', AbstractMap.SpontaneousCrashStep());
         }
         case ReadSuperblock => {
             assert AbstractMap.NextStep(Ik, Is, Is', AbstractMap.Stutter());
@@ -243,24 +171,26 @@ lemma InvImpliesRefinementNext(k:Constants, s:Variables, s':Variables)
         case ScanDiskLog => {
             assert AbstractMap.NextStep(Ik, Is, Is', AbstractMap.Stutter());
         }
-        case TerminateScan => {
-            assert DiskLogPrefix(k.disk, s.disk, |s.memlog|) == s.memlog;   // OBSERVE
-            assert AbstractMap.NextStep(Ik, Is, Is', AbstractMap.Stutter());
+        case TerminateScanStep => {
+            assert s'.memlog[..s'.diskCommittedSize] == DiskLog(k.disk, s.disk); // OBSERVE
+            assert IViewsDef(k, s', s'.diskCommittedSize, 1) == [INotRunningView(k, s)];    // OBSERVE
+            assert AbstractMap.NextStep(Ik, Is, Is', AbstractMap.Stutter()); // OBSERVE witness (Step)
         }
-        case Append(datum) => {
-            LogAppend(s.memlog, datum);
-            assert AbstractMap.NextStep(Ik, Is, Is', AbstractMap.Write(datum));
+        case AppendStep(datum) => {
+            AppendRefinement(k, s, s', datum);
         }
         case Query(datum) => {
             reveal_ILog();
             assert AbstractMap.NextStep(Ik, Is, Is', AbstractMap.Query(datum));
         }
-        case PushLogData => {
-            PushLogNoop(k.disk, s.disk, s'.disk, DiskLogSize(k.disk, s.disk));
-            assert AbstractMap.NextStep(Ik, Is, Is', AbstractMap.Stutter());
+        case PushLogDataStep => {
+            assert IViewsDef(k, s', s'.diskCommittedSize, INumRunningViews(k, s'))
+                == IViewsDef(k, s, s.diskCommittedSize, INumRunningViews(k, s)); // OBSERVE
+            assert AbstractMap.NextStep(Ik, Is, Is', AbstractMap.Stutter); // OBSERVE witness (Step)
         }
-        case PushLogMetadataStep => {
-            PushLogMetadataRefinement(k, s, s');
+        case PushLogMetadataStep(persistentCount) => {
+            var writesRetired := persistentCount - s.diskCommittedSize;
+            assert AbstractMap.NextStep(Ik, Is, Is', AbstractMap.PersistWritesStep(writesRetired)); // OBSERVE witness (Step)
         }
         case CompleteSync => {
             assert AbstractMap.NextStep(Ik, Is, Is', AbstractMap.Stutter());
